wip on splitting up behaviors

TwoState.dfy
@@ -8,6 +8,9 @@ module TwoStateModule {
     import opened util_collections_seqs_s
     import opened util_collections_seqs_i
 
+    datatype PartiallyAnnotatedBehavior<S, A> =
+        PartiallyAnnotatedBehavior(states: seq<S>, trace: seq<A>)
+
     datatype ActorTriple<S, T> = ActorTriple(s: S, s': S, actor: T)
 
     datatype YieldRequest<S(==), A(==), T(==)> = YieldPredicate(
@@ -53,7 +56,8 @@ module TwoStateModule {
     predicate StableUnderYield<S,T>(P: iset<StateActorPair<S,T>>, Y: iset<ActorTriple<S,T>>)
     {
         forall s, s', tid :: 
-            ActorTriple(s, s', tid) in Y ==> (StateActorPair(s, tid) in P <==> StateActorPair(s', tid) in P)
+            ActorTriple(s, s', tid) in Y ==>
+                (StateActorPair(s, tid) in P <==> StateActorPair(s', tid) in P)
     }
 
     // To be used once there is more than one statement
@@ -76,7 +80,11 @@ module TwoStateModule {
         forall i :: 0 <= i < |trace| ==> trace[i] in idmap && idmap[trace[i]] == tid
     }
 
-    predicate HoareLogicAssumptions<S,A,T>(r: YieldRequest<S, A, T>, their_states: seq<S>, my_states: seq<S>, trace: seq<A>)
+    predicate HoareLogicAssumptions<S,A,T>(
+        r: YieldRequest<S, A, T>,
+        their_states: seq<S>,
+        my_states: seq<S>,
+        trace: seq<A>)
     {
         && |their_states| == |my_states| == |r.pcs| == |trace| + 1
         && |trace| > 0
@@ -104,37 +112,45 @@ module TwoStateModule {
         && YieldPredicateReflexive(r.Y)
         && YieldPredicateTransitive(r.Y)
         && YieldPredicateAbstractsInterference(r.next, r.Y, r.idmap)
-        && (forall i :: 0 <= i < |r.pcs| ==> StableUnderYield(r.pcs[i], r.Y))
+//        && (forall i :: 0 <= i < |r.pcs| ==> StableUnderYield(r.pcs[i], r.Y))
         && HoareLogic(r)
     }
 
-    predicate RelyStateNextSeq<S,A,T>(next: iset<ActionTriple<S,A>>, idmap: imap<A, T>, states: seq<S>, trace: seq<A>, tid: T)
+    predicate RelyStateNextSeq<S,A,T>(
+        next: iset<ActionTriple<S,A>>,
+        idmap: imap<A, T>,
+        states: seq<S>,
+        trace: seq<A>,
+        tid: T)
     {
         && StateNextSeq(states, trace, next)
         && (forall a' :: a' in trace && a' in idmap ==> idmap[a'] != tid)
     }
 
-    predicate BehaviorLogicAssumptions<S, A, T>(r: YieldRequest<S, A, T>, states: seq<(seq<S>, seq<A>)>, trace: seq<A>)
+    predicate BehaviorLogicAssumptions<S, A, T>(
+        r: YieldRequest<S, A, T>,
+        bs: seq<PartiallyAnnotatedBehavior<S,A>>,
+        trace: seq<A>)
     {
-        && |states| == |r.pcs| == |trace| + 1
+        && |bs| == |r.pcs| == |trace| + 1
         && |trace| > 0
         && trace[0] in r.idmap
         && var tid := r.idmap[trace[0]];
         && AllActionsHaveActor(r.idmap, trace, tid)
-        && (forall i :: 0 <= i < |states| ==>
-            var (s,t) := states[i];
+        && (forall i :: 0 <= i < |bs| ==>
+            var PartiallyAnnotatedBehavior(s,t) := bs[i];
             && RelyStateNextSeq(r.next, r.idmap, s, t, tid)
             && StateActorPair(last(s), tid) in r.pcs[i])
-        && StateActorPair(states[0].0[0], tid) in r.pre
+        && StateActorPair(bs[0].states[0], tid) in r.pre
         && (forall i :: 0 <= i < |trace| ==>
-            ActionTriple(last(states[i].0), states[i+1].0[0], trace[i]) in r.next)
+            ActionTriple(last(bs[i].states), bs[i+1].states[0], trace[i]) in r.next)
     }
 
     predicate BehaviorLogic<S, A, T>(r: YieldRequest<S, A, T>)
     {
-        forall states, trace ::
-            BehaviorLogicAssumptions(r, states, trace)
-            ==> StateActorPair(last(last(states).0), r.idmap[trace[0]]) in r.post
+        forall bs, trace ::
+            BehaviorLogicAssumptions(r, bs, trace)
+            ==> StateActorPair(last(last(bs).states), r.idmap[trace[0]]) in r.post
     }
 
     lemma lemma_UseHoareLogic<S,A,T>(
@@ -175,26 +191,93 @@ module TwoStateModule {
     }
 
     lemma lemma_UseYieldPredicate<S,A,T>(
-        r: YieldRequest<S, A, T>, 
-        states: seq<(seq<S>, seq<A>)>,
+        r: YieldRequest<S, A, T>,
+        bs: seq<PartiallyAnnotatedBehavior<S,A>>,
         trace: seq<A>
         )
         requires ValidYieldRequest(r)
-        requires BehaviorLogicAssumptions(r, states, trace)
-        ensures StateActorPair(last(last(states).0), r.idmap[trace[0]]) in r.post
+        requires BehaviorLogicAssumptions(r, bs, trace)
+        ensures StateActorPair(last(last(bs).states), r.idmap[trace[0]]) in r.post
     {
         var tid := r.idmap[trace[0]];
 
-        forall i | 0 <= i < |states|
-            ensures ActorTriple(states[i].0[0], last(states[i].0), tid) in r.Y
+        forall i | 0 <= i < |bs|
+            ensures ActorTriple(bs[i].states[0], last(bs[i].states), tid) in r.Y
         {
-            var (s, t) := states[i];
+            var s := bs[i].states;
+            var t := bs[i].trace;
             lemma_YieldAbstractsNextSequence(r.next, r.Y, r.idmap, s, t, tid);
         }
 
-        var their_states := ConvertMapToSeq(|states|, map i | 0 <= i < |states| :: states[i].0[0]);
-        var my_states := ConvertMapToSeq(|states|, map i | 0 <= i < |states| :: last(states[i].0));
+        var their_states := ConvertMapToSeq(|bs|, map i | 0 <= i < |bs| :: bs[i].states[0]);
+        var my_states := ConvertMapToSeq(|bs|, map i | 0 <= i < |bs| :: last(bs[i].states));
 
         lemma_UseHoareLogic(r, their_states, my_states, trace);
     }
+
+    function AppendCompatiblePB<S, A>(
+        pb1: PartiallyAnnotatedBehavior<S, A>,
+        pb2: PartiallyAnnotatedBehavior<S, A>
+        ):
+        PartiallyAnnotatedBehavior<S, A>
+        // requires |pb2.states| > 0
+        // requires last(pb1.states) == pb2.states[0]
+    {
+        if pb2.states != [] then
+            PartiallyAnnotatedBehavior(pb1.states + pb2.states[1..], pb1.trace + pb2.trace)
+        else
+            pb1
+    }
+
+    function AppendPBWithIntermediateAction<S, A>(
+        pb1: PartiallyAnnotatedBehavior<S, A>,
+        a: A,
+        pb2: PartiallyAnnotatedBehavior<S, A>
+        ):
+        PartiallyAnnotatedBehavior<S, A>
+    {
+        PartiallyAnnotatedBehavior(pb1.states + pb2.states, pb1.trace + [a] + pb2.trace)
+    }
+
+    function ConcatPBWithIntermediateTrace<S, A>(
+        pbs: seq<PartiallyAnnotatedBehavior<S, A>>,
+        trace: seq<A>
+        ):
+        PartiallyAnnotatedBehavior<S, A>
+        requires |pbs| == |trace| + 1
+    {
+        if trace == [] then
+            pbs[0]
+        else
+            var rest := ConcatPBWithIntermediateTrace(pbs[1..], trace[1..]);
+            AppendPBWithIntermediateAction(pbs[0], trace[0], rest)
+    }
+
+
+    lemma lemma_FactorOutThreadActions<S,A,T>(
+        r: YieldRequest<S, A, T>,
+        b: PartiallyAnnotatedBehavior<S, A>,
+        tid: T
+        ) returns (
+        prefix: PartiallyAnnotatedBehavior<S,A>,
+        bs: seq<PartiallyAnnotatedBehavior<S,A>>,
+        trace: seq<A>,
+        suffix: PartiallyAnnotatedBehavior<S,A>
+        )
+        requires ValidYieldRequest(r)
+        requires StateNextSeq(b.states, b.trace, r.next)
+
+        ensures |bs| == |trace| + 1
+        ensures var middle := ConcatPBWithIntermediateTrace(bs, trace);
+            AppendCompatiblePB(prefix, AppendCompatiblePB(middle, suffix)) == b
+
+        ensures StateNextSeq(prefix.states, prefix.trace, r.next)
+        ensures BehaviorLogicAssumptions(r, bs, trace)
+        ensures StateNextSeq(suffix.states, suffix.trace, r.next)
+
+        ensures last(prefix.states) == bs[0].states[0]
+        ensures last(last(bs).states) == suffix.states[0]
+    {
+    }
+
 }
